backend/Mach.v
@@ -318,20 +318,20 @@ Inductive step: state -> trace -> state -> Prop :=
         E0 (State s vf sp c rs' m)
   | exec_Mop:
       forall s f sp op args res c rs m v rs',
-      eval_operation ge sp op rs##args m = Some v ->
+      eval_operation se sp op rs##args m = Some v ->
       rs' = ((undef_regs (destroyed_by_op op) rs)#res <- v) ->
       step (State s f sp (Mop op args res :: c) rs m)
         E0 (State s f sp c rs' m)
   | exec_Mload:
       forall s f sp chunk addr args dst c rs m a v rs',
-      eval_addressing ge sp addr rs##args = Some a ->
+      eval_addressing se sp addr rs##args = Some a ->
       Mem.loadv chunk m a = Some v ->
       rs' = ((undef_regs (destroyed_by_load chunk addr) rs)#dst <- v) ->
       step (State s f sp (Mload chunk addr args dst :: c) rs m)
         E0 (State s f sp c rs' m)
   | exec_Mstore:
       forall s f sp chunk addr args src c rs m m' a rs',
-      eval_addressing ge sp addr rs##args = Some a ->
+      eval_addressing se sp addr rs##args = Some a ->
       Mem.storev chunk m a (rs src) = Some m' ->
       rs' = undef_regs (destroyed_by_store chunk addr) rs ->
       step (State s f sp (Mstore chunk addr args src :: c) rs m)
